WIP on scmem properties with older proofs skipped

Kami/Ex/Trace.v
@@ -129,7 +129,7 @@ Section AbstractTrace.
       -> censorTrace tr1 = censorTrace tr2
       -> (tr1 = nil /\ tr2 = nil)
         \/ pc1 = pc2.
-  Proof.
+  Proof. (*
     intros ? ? ? ? ? ? ? ? ? ? Hht1 Hht2 Hct.
     inversion Hht1; inversion Hht2;
       intros; subst; try tauto; right;
@@ -161,7 +161,7 @@ Section AbstractTrace.
                          remember x as x' eqn:Heq; clear - Hct
                        end
             end; inversion Hct; congruence.
-    Qed.
+    Qed. *) Admitted.
 
   Definition extractFhTrace : list TraceEvent -> list data :=
     flat_map (fun te => match te with
@@ -330,6 +330,9 @@ Ltac shatter := repeat match goal with
 
 Section SCTiming.
 
+  Definition rv32iRq := RqFromProc rv32iAddrSize rv32iDataBytes.
+  Definition rv32iRs := RsToProc rv32iDataBytes.
+
   Definition rv32iProcInst :=
     procInst rv32iGetOptype
              rv32iGetLdDst rv32iGetLdAddr rv32iGetLdSrc rv32iCalcLdAddr
@@ -401,8 +404,8 @@ Section SCTiming.
                                             "op" :: Bool;
                                             "data" :: Bit 32});
                      ret := Struct (STRUCT {"data" :: Bit 32}) |}
-                  (evalExpr (STRUCT { "addr" ::= #argV!(RqFromProc rv32iAddrSize rv32iDataBytes)@."addr";
-                                      "op" ::= #argV!(RqFromProc rv32iAddrSize rv32iDataBytes)@."op";
+                  (evalExpr (STRUCT { "addr" ::= #argV!rv32iRq@."addr";
+                                      "op" ::= #argV!rv32iRq@."op";
                                       "data" ::= $0 })%kami_expr,
                    evalExpr (STRUCT { "data" ::= $0 })%kami_expr)
          | _ => t
@@ -455,10 +458,10 @@ Section SCTiming.
                                                  "data" :: Bit 32});
                           ret := Struct (STRUCT {"data" :: Bit 32}) |}
                        (argV, retV)) =>
-          let addr := evalExpr (#argV!(RqFromProc rv32iAddrSize rv32iDataBytes)@."addr")%kami_expr in
-          let argval := evalExpr (#argV!(RqFromProc rv32iAddrSize rv32iDataBytes)@."data")%kami_expr in
-          let retval := evalExpr (#retV!(RsToProc rv32iDataBytes)@."data")%kami_expr in
-          if evalExpr (#argV!(RqFromProc rv32iAddrSize rv32iDataBytes)@."op")%kami_expr
+          let addr := evalExpr (#argV!rv32iRq@."addr")%kami_expr in
+          let argval := evalExpr (#argV!rv32iRq@."data")%kami_expr in
+          let retval := evalExpr (#retV!rv32iRs@."data")%kami_expr in
+          if evalExpr (#argV!rv32iRq@."op")%kami_expr
           then Some (Wr $0 addr argval)
           else Some (Rd $0 addr retval)
         | _ => None
@@ -509,7 +512,7 @@ Section SCTiming.
   Lemma relatedFhTrace :
     forall trace ls,
       relatedTrace trace ls -> extractFhTrace trace = extractFhLabelSeq ls.
-  Proof.
+  Proof. (*
     induction 1; try eauto;
       simpl;
       match goal with
@@ -531,7 +534,7 @@ Section SCTiming.
     | [ H : Some _ = Some _ |- _ ] => inversion H
     end.
     reflexivity.
-  Qed.
+  Qed. *) Admitted.
 
   Inductive SCProcMemConsistent : LabelSeqT -> memory -> Prop :=
   | SPMCnil : forall mem, SCProcMemConsistent nil mem
@@ -543,10 +546,10 @@ Section SCTiming.
                                                "data" :: Bit 32});
                         ret := Struct (STRUCT {"data" :: Bit 32}) |}
                      (argV, retV)) =>
-        let addr := evalExpr (#argV!(RqFromProc rv32iAddrSize rv32iDataBytes)@."addr")%kami_expr in
-        let argval := evalExpr (#argV!(RqFromProc rv32iAddrSize rv32iDataBytes)@."data")%kami_expr in
-        let retval := evalExpr (#retV!(RsToProc rv32iDataBytes)@."data")%kami_expr in
-        if evalExpr (#argV!(RqFromProc rv32iAddrSize rv32iDataBytes)@."op")%kami_expr
+        let addr := evalExpr (#argV!rv32iRq@."addr")%kami_expr in
+        let argval := evalExpr (#argV!rv32iRq@."data")%kami_expr in
+        let retval := evalExpr (#retV!rv32iRs@."data")%kami_expr in
+        if evalExpr (#argV!rv32iRq@."op")%kami_expr
         then mem' = (fun a => if weq a addr then argval else mem a)
         else mem addr = retval /\ mem' = mem
       | _ => mem' = mem
@@ -573,7 +576,7 @@ Section SCTiming.
            | [ Heq : ?x = ?y |- _ ] => ((tryif unfold x then fail else subst x) || (tryif unfold y then fail else subst y))
            end.
 
-  Lemma SCSubsteps :
+  Lemma SCProcSubsteps :
     forall o (ss : Substeps rv32iProcInst o),
       SubstepsInd rv32iProcInst o (foldSSUpds ss) (foldSSLabel ss) ->
       (((foldSSLabel ss) = {| annot := None; defs := FMap.M.empty _; calls := FMap.M.empty _ |}
@@ -584,7 +587,7 @@ Section SCTiming.
             /\ SemAction o (a type) u cs WO
             /\ (foldSSLabel ss) = {| annot := Some (Some k); defs := FMap.M.empty _; calls := cs |}
             /\ (foldSSUpds ss) = u).
-  Proof.
+  Proof. (*
     intros.
     match goal with
     | [ H : SubstepsInd _ _ _ _ |- _ ] => induction H
@@ -615,7 +618,7 @@ Section SCTiming.
             simpl;
             FMap.findeq
         end.
-  Qed.
+  Qed. *) Admitted.
 
   Ltac evex H := unfold evalExpr in H; fold evalExpr in H.
   Ltac evexg := unfold evalExpr; fold evalExpr.
@@ -687,7 +690,7 @@ Section SCTiming.
       relatedTrace trace2 ls2 ->
       censorTrace trace1 = censorTrace trace2 ->
       censorLabelSeq censorSCMeth ls1 = censorLabelSeq censorSCMeth ls2.
-  Proof.
+  Proof. (*
     intros rf1 rf2 pm pc mem1 mem2 trace1 trace2 newRegs1 newRegs2 ls1 ls2 Hht1.
     move Hht1 at top.
     generalize rf2 mem2 trace2 newRegs1 newRegs2 ls1 ls2.
@@ -728,7 +731,7 @@ Section SCTiming.
              end.
       opaque_subst.
       apply substepsComb_substepsInd in HSubsteps.
-      apply SCSubsteps in HSubsteps.
+      apply SCProcSubsteps in HSubsteps.
       intuition idtac; shatter;
         match goal with
         | [ H : foldSSLabel ss = _, H1 : annot (hide (foldSSLabel ss)) = None -> False, H2 : annot (hide (foldSSLabel ss)) = Some None -> False |- _ ] => rewrite H in *; simpl in H1; simpl in H2; try tauto
@@ -740,7 +743,7 @@ Section SCTiming.
       intuition idtac; kinv_action_dest; SCRegs_find; expr_equalities; try tauto; try discriminate.
       Transparent evalExpr.
       apply substepsComb_substepsInd in HSubsteps0.
-      apply SCSubsteps in HSubsteps0.
+      apply SCProcSubsteps in HSubsteps0.
       intuition idtac; shatter;
         match goal with
         | [ H : foldSSLabel ss0 = _, H1 : annot (hide (foldSSLabel ss0)) = None -> False, H2 : annot (hide (foldSSLabel ss0)) = Some None -> False |- _ ] => rewrite H in *; simpl in H1; simpl in H2; try tauto
@@ -772,7 +775,7 @@ Section SCTiming.
           | [ H : labelToTraceEvent ?l = _,
                   x : forall _ : Fin.t 1, _
                                      |- _ = evalExpr ?adr ] =>
-            replace (labelToTraceEvent l) with (Some (Rd $ (0) (evalExpr adr) (evalExpr (#x!(RsToProc rv32iDataBytes)@."data")%kami_expr))) in H by eauto
+            replace (labelToTraceEvent l) with (Some (Rd $ (0) (evalExpr adr) (evalExpr (#x!rv32iRs@."data")%kami_expr))) in H by eauto
           end.
           Opaque evalExpr.
           match goal with
@@ -851,7 +854,7 @@ Section SCTiming.
                                         |- _ ] =>
                match goal with
                | [ H : labelToTraceEvent (hide {| annot := _; defs := _; calls := FMap.M.add _ (existT _ _ (evalExpr STRUCT {"addr" ::= ?adr; "op" ::= _; "data" ::= _}%kami_expr, x)) _|}) = Some (Rd $ (0) _ (mem laddr_aligned)) |- _ ] =>
-                 replace (labelToTraceEvent l) with (Some (Rd $ (0) (evalExpr adr) (evalExpr (#x!(RsToProc rv32iDataBytes)@."data")%kami_expr))) in H by eauto; inversion H
+                 replace (labelToTraceEvent l) with (Some (Rd $ (0) (evalExpr adr) (evalExpr (#x!rv32iRs@."data")%kami_expr))) in H by eauto; inversion H
                end
              end.
              reflexivity.
@@ -893,7 +896,7 @@ Section SCTiming.
                                         |- _ ] =>
                match goal with
                | [ H : labelToTraceEvent (hide {| annot := _; defs := _; calls := FMap.M.add _ (existT _ _ (evalExpr STRUCT {"addr" ::= ?adr; "op" ::= _; "data" ::= _}%kami_expr, x)) _|}) = Some (Rd $ (0) _ val0) |- _ ] =>
-                 replace (labelToTraceEvent l) with (Some (Rd $ (0) (evalExpr adr) (evalExpr (#x!(RsToProc rv32iDataBytes)@."data")%kami_expr))) in H
+                 replace (labelToTraceEvent l) with (Some (Rd $ (0) (evalExpr adr) (evalExpr (#x!rv32iRs@."data")%kami_expr))) in H
                end
              end.
              ++ Opaque evalExpr.
@@ -968,7 +971,7 @@ Section SCTiming.
              end.
       opaque_subst.
       apply substepsComb_substepsInd in HSubsteps.
-      apply SCSubsteps in HSubsteps.
+      apply SCProcSubsteps in HSubsteps.
       intuition idtac; shatter;
         match goal with
         | [ H : foldSSLabel ss = _, H1 : annot (hide (foldSSLabel ss)) = None -> False, H2 : annot (hide (foldSSLabel ss)) = Some None -> False |- _ ] => rewrite H in *; simpl in H1; simpl in H2; try tauto
@@ -980,7 +983,7 @@ Section SCTiming.
       intuition idtac; kinv_action_dest; SCRegs_find; expr_equalities; try tauto; try discriminate.
       Transparent evalExpr.
       + apply substepsComb_substepsInd in HSubsteps0.
-        apply SCSubsteps in HSubsteps0.
+        apply SCProcSubsteps in HSubsteps0.
         intuition idtac; shatter;
           match goal with
           | [ H : foldSSLabel ss0 = _, H1 : annot (hide (foldSSLabel ss0)) = None -> False, H2 : annot (hide (foldSSLabel ss0)) = Some None -> False |- _ ] => rewrite H in *; simpl in H1; simpl in H2; try tauto
@@ -1099,7 +1102,7 @@ Section SCTiming.
              end.
       opaque_subst.
       apply substepsComb_substepsInd in HSubsteps.
-      apply SCSubsteps in HSubsteps.
+      apply SCProcSubsteps in HSubsteps.
       intuition idtac; shatter;
         match goal with
         | [ H : foldSSLabel ss = _, H1 : annot (hide (foldSSLabel ss)) = None -> False, H2 : annot (hide (foldSSLabel ss)) = Some None -> False |- _ ] => rewrite H in *; simpl in H1; simpl in H2; try tauto
@@ -1111,7 +1114,7 @@ Section SCTiming.
       intuition idtac; kinv_action_dest; SCRegs_find; expr_equalities; try tauto; try discriminate.
       Transparent evalExpr.
       apply substepsComb_substepsInd in HSubsteps0.
-      apply SCSubsteps in HSubsteps0.
+      apply SCProcSubsteps in HSubsteps0.
       intuition idtac; shatter;
         match goal with
         | [ H : foldSSLabel ss0 = _, H1 : annot (hide (foldSSLabel ss0)) = None -> False, H2 : annot (hide (foldSSLabel ss0)) = Some None -> False |- _ ] => rewrite H in *; simpl in H1; simpl in H2; try tauto
@@ -1298,7 +1301,7 @@ Section SCTiming.
              end.
       opaque_subst.
       apply substepsComb_substepsInd in HSubsteps.
-      apply SCSubsteps in HSubsteps.
+      apply SCProcSubsteps in HSubsteps.
       intuition idtac; shatter;
         match goal with
         | [ H : foldSSLabel ss = _, H1 : annot (hide (foldSSLabel ss)) = None -> False, H2 : annot (hide (foldSSLabel ss)) = Some None -> False |- _ ] => rewrite H in *; simpl in H1; simpl in H2; try tauto
@@ -1310,7 +1313,7 @@ Section SCTiming.
       intuition idtac; kinv_action_dest; SCRegs_find; expr_equalities; try tauto; try discriminate.
       Transparent evalExpr.
       apply substepsComb_substepsInd in HSubsteps0.
-      apply SCSubsteps in HSubsteps0.
+      apply SCProcSubsteps in HSubsteps0.
       intuition idtac; shatter;
         match goal with
         | [ H : foldSSLabel ss0 = _, H1 : annot (hide (foldSSLabel ss0)) = None -> False, H2 : annot (hide (foldSSLabel ss0)) = Some None -> False |- _ ] => rewrite H in *; simpl in H1; simpl in H2; try tauto
@@ -1435,7 +1438,7 @@ Section SCTiming.
              end.
       opaque_subst.
       apply substepsComb_substepsInd in HSubsteps.
-      apply SCSubsteps in HSubsteps.
+      apply SCProcSubsteps in HSubsteps.
       intuition idtac; shatter;
         match goal with
         | [ H : foldSSLabel ss = _, H1 : annot (hide (foldSSLabel ss)) = None -> False, H2 : annot (hide (foldSSLabel ss)) = Some None -> False |- _ ] => rewrite H in *; simpl in H1; simpl in H2; try tauto
@@ -1447,7 +1450,7 @@ Section SCTiming.
       intuition idtac; kinv_action_dest; SCRegs_find; expr_equalities; try tauto; try discriminate.
       Transparent evalExpr.
       + apply substepsComb_substepsInd in HSubsteps0.
-        apply SCSubsteps in HSubsteps0.
+        apply SCProcSubsteps in HSubsteps0.
         intuition idtac; shatter;
           match goal with
           | [ H : foldSSLabel ss0 = _, H1 : annot (hide (foldSSLabel ss0)) = None -> False, H2 : annot (hide (foldSSLabel ss0)) = Some None -> False |- _ ] => rewrite H in *; simpl in H1; simpl in H2; try tauto
@@ -1574,7 +1577,7 @@ Section SCTiming.
              subst.
              assumption.
       + apply substepsComb_substepsInd in HSubsteps0.
-        apply SCSubsteps in HSubsteps0.
+        apply SCProcSubsteps in HSubsteps0.
         intuition idtac; shatter;
           match goal with
           | [ H : foldSSLabel ss0 = _, H1 : annot (hide (foldSSLabel ss0)) = None -> False, H2 : annot (hide (foldSSLabel ss0)) = Some None -> False |- _ ] => rewrite H in *; simpl in H1; simpl in H2; try tauto
@@ -1706,7 +1709,7 @@ Section SCTiming.
                end.
         opaque_subst.
         apply substepsComb_substepsInd in HSubsteps.
-        apply SCSubsteps in HSubsteps.
+        apply SCProcSubsteps in HSubsteps.
         intuition idtac; shatter;
           match goal with
           | [ H : foldSSLabel ss = _, H1 : annot (hide (foldSSLabel ss)) = None -> False, H2 : annot (hide (foldSSLabel ss)) = Some None -> False |- _ ] => rewrite H in *; simpl in H1; simpl in H2; try tauto
@@ -1726,7 +1729,7 @@ Section SCTiming.
           end.
           tauto.
         * apply substepsComb_substepsInd in HSubsteps0.
-          apply SCSubsteps in HSubsteps0.
+          apply SCProcSubsteps in HSubsteps0.
           intuition idtac; shatter;
             match goal with
             | [ H : foldSSLabel ss0 = _, H1 : annot (hide (foldSSLabel ss0)) = None -> False, H2 : annot (hide (foldSSLabel ss0)) = Some None -> False |- _ ] => rewrite H in *; simpl in H1; simpl in H2; try tauto
@@ -1823,7 +1826,7 @@ Section SCTiming.
                end.
         opaque_subst.
         apply substepsComb_substepsInd in HSubsteps.
-        apply SCSubsteps in HSubsteps.
+        apply SCProcSubsteps in HSubsteps.
         intuition idtac; shatter;
           match goal with
           | [ H : foldSSLabel ss = _, H1 : annot (hide (foldSSLabel ss)) = None -> False, H2 : annot (hide (foldSSLabel ss)) = Some None -> False |- _ ] => rewrite H in *; simpl in H1; simpl in H2; try tauto
@@ -1843,7 +1846,7 @@ Section SCTiming.
           end.
           tauto.
         * apply substepsComb_substepsInd in HSubsteps0.
-          apply SCSubsteps in HSubsteps0.
+          apply SCProcSubsteps in HSubsteps0.
           intuition idtac; shatter;
             match goal with
             | [ H : foldSSLabel ss0 = _, H1 : annot (hide (foldSSLabel ss0)) = None -> False, H2 : annot (hide (foldSSLabel ss0)) = Some None -> False |- _ ] => rewrite H in *; simpl in H1; simpl in H2; try tauto
@@ -1940,7 +1943,7 @@ Section SCTiming.
              end.
       opaque_subst.
       apply substepsComb_substepsInd in HSubsteps.
-      apply SCSubsteps in HSubsteps.
+      apply SCProcSubsteps in HSubsteps.
       intuition idtac; shatter;
         match goal with
         | [ H : foldSSLabel ss = _, H1 : annot (hide (foldSSLabel ss)) = None -> False, H2 : annot (hide (foldSSLabel ss)) = Some None -> False |- _ ] => rewrite H in *; simpl in H1; simpl in H2; try tauto
@@ -1956,7 +1959,7 @@ Section SCTiming.
         end.
         discriminate.
       + apply substepsComb_substepsInd in HSubsteps0.
-        apply SCSubsteps in HSubsteps0.
+        apply SCProcSubsteps in HSubsteps0.
         intuition idtac; shatter;
           match goal with
           | [ H : foldSSLabel ss0 = _, H1 : annot (hide (foldSSLabel ss0)) = None -> False, H2 : annot (hide (foldSSLabel ss0)) = Some None -> False |- _ ] => rewrite H in *; simpl in H1; simpl in H2; try tauto
@@ -2033,7 +2036,7 @@ Section SCTiming.
           subst.
           assumption.
       + apply substepsComb_substepsInd in HSubsteps0.
-        apply SCSubsteps in HSubsteps0.
+        apply SCProcSubsteps in HSubsteps0.
         intuition idtac; shatter;
           match goal with
           | [ H : foldSSLabel ss0 = _, H1 : annot (hide (foldSSLabel ss0)) = None -> False, H2 : annot (hide (foldSSLabel ss0)) = Some None -> False |- _ ] => rewrite H in *; simpl in H1; simpl in H2; try tauto
@@ -2109,7 +2112,7 @@ Section SCTiming.
           Transparent evalExpr.
           subst.
           assumption.
-  Qed.
+  Qed. *) Admitted.
 
   Lemma eval_const : forall n (t : Expr type (SyntaxKind (Bit n))) c, evalExpr t = c -> evalExpr (t == (Const _ (ConstBit c)))%kami_expr = true.
     simpl.
@@ -2125,7 +2128,7 @@ Section SCTiming.
         ForwardActiveMultistep rv32iProcInst (SCRegs rf pm pc) newRegs ls /\
         SCProcMemConsistent ls mem /\
         relatedTrace trace ls.
-  Proof.
+  Proof. (* 
     induction 1.
     - repeat eexists; repeat econstructor.
     - shatter.
@@ -2561,7 +2564,7 @@ Section SCTiming.
           Unshelve.
           -- exact (evalExpr (STRUCT { "data" ::= $0 }))%kami_expr.
           -- exact (wzero _).
-  Qed.
+  Qed. *) Admitted.
 
   Definition getrf (regs : RegsT) : regfile :=
     match FMap.M.find "rf" regs with
@@ -2594,7 +2597,7 @@ Section SCTiming.
       exists trace,
         hasTrace rf pm pc mem trace /\
         relatedTrace trace ls.
-  Proof.
+  Proof. (*
     intros rf pm pc mem newRegs ls Hfm Hmem.
     let Heq := fresh in
     remember (SCRegs rf pm pc) as regs eqn:Heq; unfold SCRegs in Heq;
@@ -2611,7 +2614,7 @@ Section SCTiming.
       | [ H : Step _ _ _ _ |- _ ] => destruct H
       end.
       apply substepsComb_substepsInd in HSubsteps.
-      apply SCSubsteps in HSubsteps.
+      apply SCProcSubsteps in HSubsteps.
       intuition idtac; shatter;
         match goal with
         | [ Hle : foldSSLabel ss = _, Hue : foldSSUpds ss = _ |- _ ] => rewrite Hle in *; rewrite Hue in *
@@ -3154,7 +3157,7 @@ Section SCTiming.
                 end.
           -- constructor; try assumption.
              FMap.findeq.
-  Qed.
+  Qed. *) Admitted.
 
   Theorem abstractToSCProcHiding :
     forall rf pm pc mem,
@@ -3194,6 +3197,89 @@ Section SCTiming.
       end.
   Qed.
 
+  Definition rv32iMemInstExec {ty} : ty (Struct rv32iRq) -> ActionT ty (Struct rv32iRs) :=
+    fun (a: ty (Struct rv32iRq)) =>
+      (If !#a!rv32iRq@."op" then (* load *)
+         Read memv <- "mem";
+         LET ldval <- #memv@[#a!rv32iRq@."addr"];
+         Ret (STRUCT { "data" ::= #ldval } :: Struct rv32iRs)
+       else (* store *)
+         Read memv <- "mem";
+         Write "mem" <- #memv@[ #a!rv32iRq@."addr" <- #a!rv32iRq@."data" ];
+         Ret (STRUCT { "data" ::= $$Default } :: Struct rv32iRs)
+       as na;
+       Ret #na)%kami_action.
+  
+  Definition rv32iMemInstSingle := MODULE {
+    Register "mem" : Vector (MemTypes.Data rv32iDataBytes) rv32iAddrSize <- Default
+
+    with Method "exec" (a : Struct rv32iRq) : Struct rv32iRs := (rv32iMemInstExec a)
+  }.
+
+  Lemma SCMemSubsteps :
+    forall o (ss : Substeps rv32iMemInstSingle o),
+      SubstepsInd rv32iMemInstSingle o (foldSSUpds ss) (foldSSLabel ss) ->
+      (((foldSSLabel ss) = {| annot := None; defs := FMap.M.empty _; calls := FMap.M.empty _ |}
+        \/ (foldSSLabel ss) = {| annot := Some None; defs := FMap.M.empty _; calls := FMap.M.empty _ |})
+       /\ (foldSSUpds ss) = FMap.M.empty _)
+      \/ (exists argV retV u,
+            SemAction o (rv32iMemInstExec argV) u (FMap.M.empty _) retV
+            /\ (foldSSLabel ss) = {| annot := None; defs := FMap.M.add "exec" (existT _
+                       {| arg := Struct (STRUCT {"addr" :: Bit 16;
+                                                 "op" :: Bool;
+                                                 "data" :: Bit 32});
+                          ret := Struct (STRUCT {"data" :: Bit 32}) |}
+                       (argV, retV)) (FMap.M.empty _); calls := FMap.M.empty _ |}
+            /\ (foldSSUpds ss) = u).
+  Proof.
+    intros.
+    match goal with
+    | [ H : SubstepsInd _ _ _ _ |- _ ] => induction H
+    end.
+    - tauto.
+    - intuition idtac;
+        simpl;
+        shatter;
+        intuition idtac;
+        subst;
+        match goal with
+        | [ H : Substep _ _ _ _ _ |- _ ] => destruct H
+        end;
+        try tauto;
+        match goal with
+        | [ HIn : In _ (getRules rv32iMemInstSingle) |- _ ] => simpl in HIn; tauto
+        | _ => idtac
+        end.
+      + right.
+        simpl in HIn.
+        intuition idtac.
+        subst.
+        simpl in *.
+        exists argV, retV, u.
+        replace cs with (FMap.M.empty {x : SignatureT & SignT x}) in *.
+        * intuition idtac.
+        * kinv_action_dest; FMap.findeq.
+      + 
+      + 
+        match goal with
+        | [ HCCU : CanCombineUUL _ {| annot := Some _; defs := FMap.M.empty _; calls := _ |} _ _ (Rle _) |- _ ] =>
+          unfold CanCombineUUL in HCCU;
+            simpl in HCCU;
+            tauto
+        | [ HIn : In _ (getDefsBodies rv32iProcInst) |- _ ] =>
+          simpl in HIn;
+            tauto
+        | [ HIR : In (?k :: ?a)%struct _, HA : SemAction _ _ ?u ?cs _ |- _ ] =>
+          right;
+            exists k, a, u, cs;
+            simpl in HIR;
+            intuition idtac;
+            simpl;
+            FMap.findeq
+        end.
+  Qed.
+
+  Definition SCMemHiding
 End SCTiming.
 
 Section ThreeStageTiming.
@@ -3261,8 +3347,8 @@ Section ThreeStageTiming.
                                             "op" :: Bool;
                                             "data" :: Bit 32});
                      ret := Bit 0 |}
-                  (evalExpr (STRUCT { "addr" ::= #argV!(RqFromProc rv32iAddrSize rv32iDataBytes)@."addr";
-                                      "op" ::= #argV!(RqFromProc rv32iAddrSize rv32iDataBytes)@."op";
+                  (evalExpr (STRUCT { "addr" ::= #argV!rv32iRq@."addr";
+                                      "op" ::= #argV!rv32iRq@."op";
                                       "data" ::= $0 })%kami_expr,
                    $0)
          | _ => t
